Modularise functional-big-step semantics

src/Core_Erlang_Functional_Big_Step.v
@@ -39,13 +39,28 @@ Inductive MapResultType : Type :=
 | MapTimeout
 | MapFailure.
 
-Fixpoint fbs_expr (env : Environment) (id : nat) (expr : Expression) (eff : SideEffectList) (clock : nat) {struct clock} : ResultType :=
+Fixpoint fbs_values {A : Type} (f : Environment -> nat -> A -> SideEffectList -> ResultType) (env : Environment) (id : nat) (exps : list A) (eff : SideEffectList) : ResultType :=
+match exps with
+| []    => Result id (inl []) eff
+| x::xs => match f env id x eff with
+          | Result id' (inl [v]) eff' => 
+            let res := fbs_values f env id' xs eff' in
+              match res with
+              | Result id'' (inl xs') eff'' => Result id'' (inl (v::xs')) eff''
+              | r => r
+              end
+          | Result id' (inl val) eff' => Failure (* undefined behaviour *)
+          | r => r
+          end
+end.
+
+Fixpoint fbs_expr (clock : nat) (env : Environment) (id : nat) (expr : Expression) (eff : SideEffectList) {struct clock} : ResultType :=
 match clock with
 | 0 => Timeout
 | S clock' =>
   match expr with
    | EValues el => 
-       (fix eval_list env id exps eff : ResultType := 
+       (* (fix eval_list env id exps eff : ResultType := 
                    match exps with
                    | []    => Result id (inl []) eff
                    | x::xs => match fbs_single env id x eff clock' with
@@ -59,11 +74,12 @@ match clock with
                               | r => r
                               end
                    end
-                   ) env id el eff
-   | ESingle e => fbs_single env id e eff clock'
+                   ) *) 
+                   fbs_values (fbs_single clock') env id el eff
+   | ESingle e => fbs_single clock' env id e eff
   end
 end
-with fbs_single (env : Environment) (id : nat) (expr : SingleExpression) (eff : SideEffectList) (clock : nat) {struct clock} : ResultType :=
+with fbs_single (clock : nat) (env : Environment) (id : nat) (expr : SingleExpression) (eff : SideEffectList) {struct clock} : ResultType :=
 match clock with
 | 0 => Timeout
 | S clock' =>
@@ -74,9 +90,9 @@ match clock with
    | EFunId f => Result id (get_value env (inr f)) eff
    | EFun vl e => Result (S id) (inl [VClos env [] id vl e]) eff
    | ECons hd tl => 
-     match fbs_expr env id hd eff clock' with
+     match fbs_expr clock' env id hd eff with
        | Result id' (inl [hdv]) eff' =>
-         match fbs_expr env id' tl eff' clock' with
+         match fbs_expr clock' env id' tl eff' with
          | Result id'' (inl [tlv]) eff'' => Result id'' (inl [VCons hdv tlv]) eff''
          | Result id'' (inl val) eff'' => Failure (* undefined behaviour *)
          | r => r
@@ -85,97 +101,33 @@ match clock with
        | r => r
      end
    | ETuple l =>
-     let res := 
-     (fix eval_list env id exps eff : ResultType := 
-         match exps with
-         | []    => Result id (inl []) eff
-         | x::xs => match fbs_expr env id x eff clock' with
-                    | Result id' (inl [v]) eff' => 
-                      let res := eval_list env id' xs eff' in
-                        match res with
-                        | Result id'' (inl xs') eff'' => Result id'' (inl (v::xs')) eff''
-                        | r => r
-                        end
-                    | Result id' (inl val) eff' => Failure (* undefined behaviour *)
-                    | r => r
-                    end
-         end
-         ) env id l eff
-       in
+     let res := fbs_values (fbs_expr clock') env id l eff in
        match res with
        | Result id' (inl vl) eff' => Result id' (inl [VTuple vl]) eff'
        | r => r
        end
    | ECall f l => 
-     let res := 
-     (fix eval_list env id exps eff : ResultType := 
-         match exps with
-         | []    => Result id (inl []) eff
-         | x::xs => match fbs_expr env id x eff clock' with
-                    | Result id' (inl [v]) eff' => 
-                      let res := eval_list env id' xs eff' in
-                        match res with
-                        | Result id'' (inl xs') eff'' => Result id'' (inl (v::xs')) eff''
-                        | r => r
-                        end
-                    | Result id' (inl val) eff' => Failure (* undefined behaviour *)
-                    | r => r
-                    end
-         end
-         ) env id l eff
-       in
+     let res := fbs_values (fbs_expr clock') env id l eff in
        match res with
        | Result id' (inl vl) eff' => let (x, y) := eval f vl eff' in Result id' x y
        | r => r
        end
    | EPrimOp f l =>
-     let res := 
-     (fix eval_list env id exps eff : ResultType := 
-         match exps with
-         | []    => Result id (inl []) eff
-         | x::xs => match fbs_expr env id x eff clock' with
-                    | Result id' (inl [v]) eff' => 
-                      let res := eval_list env id' xs eff' in
-                        match res with
-                        | Result id'' (inl xs') eff'' => Result id'' (inl (v::xs')) eff''
-                        | r => r
-                        end
-                    | Result id' (inl val) eff' => Failure (* undefined behaviour *)
-                    | r => r
-                    end
-         end
-         ) env id l eff
-       in
+     let res := fbs_values (fbs_expr clock') env id l eff in
        match res with
        | Result id' (inl vl) eff' => let (x, y) := eval f vl eff' in Result id' x y
        | r => r
        end
    | EApp exp l =>
-     match fbs_expr env id exp eff clock' with
+     match fbs_expr clock' env id exp eff with
      | Result id' (inl [v]) eff' =>
-       let res := 
-       (fix eval_list env id exps eff : ResultType := 
-         match exps with
-         | []    => Result id (inl []) eff
-         | x::xs => match fbs_expr env id x eff clock' with
-                    | Result id' (inl [v]) eff' => 
-                      let res := eval_list env id' xs eff' in
-                        match res with
-                        | Result id'' (inl xs') eff'' => Result id'' (inl (v::xs')) eff''
-                        | r => r
-                        end
-                    | Result id' (inl val) eff' => Failure (* undefined behaviour *)
-                    | r => r
-                    end
-         end
-         ) env id' l eff'
-         in
+       let res := fbs_values (fbs_expr clock') env id' l eff' in
          match res with
          | Result id'' (inl vl) eff'' => 
            match v with
            | VClos ref ext closid varl body =>
               if Nat.eqb (length varl) (length vl)
-              then fbs_expr (append_vars_to_env varl vl (get_env ref ext)) id'' body eff'' clock'
+              then fbs_expr clock' (append_vars_to_env varl vl (get_env ref ext)) id'' body eff''
               else Result id'' (inr (badarity v)) eff''
            | _ => Result id'' (inr (badfun v)) eff''
            end
@@ -185,7 +137,7 @@ match clock with
      | r => r
      end
    | ECase e l =>
-     match fbs_expr env id e eff clock' with
+     match fbs_expr clock' env id e eff with
      | Result id' (inl vals) eff' =>
        (fix clause_eval l i' :=
          let i := (length l) - i' in
@@ -195,12 +147,12 @@ match clock with
            (* TODO: side effects cannot be produced here *)
              match match_clause vals l i with
              | Some (gg, bb, bindings) =>
-               match fbs_expr (add_bindings bindings env) id' gg eff' clock' with
+               match fbs_expr clock' (add_bindings bindings env) id' gg eff' with
                | Result id'' (inl [v]) eff'' =>  
                    match v with
                    | VLit (Atom "true"%string)  => 
                       if andb (Nat.eqb id'' id') (list_eqb effect_eqb eff' eff'')
-                      then fbs_expr (add_bindings bindings env) id' bb eff' clock'
+                      then fbs_expr clock' (add_bindings bindings env) id' bb eff'
                       else (* undef *) Failure
                    | VLit (Atom "false"%string) => clause_eval l i''
                    | _ => Failure
@@ -214,29 +166,39 @@ match clock with
      | r => r
      end
    | ELet l e1 e2 =>
-      match fbs_expr env id e1 eff clock' with
+      match fbs_expr clock' env id e1 eff with
       | Result id' (inl vals) eff' =>
         if Nat.eqb (length vals) (length l)
-        then fbs_expr (append_vars_to_env l vals env) id' e2 eff' clock'
+        then fbs_expr clock' (append_vars_to_env l vals env) id' e2 eff'
         else Failure
       | r => r
       end
    | ESeq e1 e2 =>
-      match fbs_expr env id e1 eff clock' with
-      | Result id' (inl [v]) eff' => fbs_expr env id' e2 eff' clock'
+      match fbs_expr clock' env id e1 eff with
+      | Result id' (inl [v]) eff' => fbs_expr clock' env id' e2 eff'
       | Result id' (inl vals) eff' => Failure
       | r => r
       end
-   | ELetRec l e => fbs_expr (append_funs_to_env l env id) (id + length l) e eff clock'
+   | ELetRec l e => fbs_expr clock' (append_funs_to_env l env id) (id + length l) e eff
    | EMap l =>
-     let res :=
-     (fix eval_list_map env id exps eff : MapResultType :=
+     let res := fbs_values (fbs_expr clock') env id (make_map_exps l) eff in
+       match res with
+       | Result id' (inl vals) eff' => 
+         match make_map_vals_inverse vals with
+         | None => Failure
+         | Some (kvals, vvals) =>
+           let (x, y) := make_value_map kvals vvals in 
+             Result id' (inl [VMap (combine x y)]) eff'
+         end
+       | r => r
+       end
+     (* (fix eval_list_map env id exps eff : MapResultType :=
        match exps with
        | [] => MapResult id (inl ([], [])) eff
        | (key, val)::xs =>
-         match fbs_expr env id key eff clock' with
+         match fbs_expr clock' env id key eff with
          | Result id' (inl [kval]) eff' =>
-            match fbs_expr env id' val eff' clock' with
+            match fbs_expr clock' env id' val eff' with
             | Result id'' (inl [vval]) eff'' => 
                let res := eval_list_map env id'' xs eff''
                in match res with
@@ -263,15 +225,15 @@ match clock with
      | MapResult id' (inr ex) eff' => Result id' (inr ex) eff'
      | MapFailure => Failure
      | MapTimeout => Timeout
-     end
+     end *)
    | ETry e1 vl1 e2 vl2 e3 =>
-     match fbs_expr env id e1 eff clock' with
+     match fbs_expr clock' env id e1 eff with
      | Result id' (inl vals) eff' =>
        if Nat.eqb (length vals) (length vl1)
-       then fbs_expr (append_vars_to_env vl1 vals env) id' e2 eff' clock'
+       then fbs_expr clock' (append_vars_to_env vl1 vals env) id' e2 eff'
        else Failure
      | Result id' (inr ex) eff' =>
-       fbs_expr (append_try_vars_to_env vl2 [exclass_to_value (fst (fst ex)); snd (fst ex); snd ex] env) id' e3 eff' clock'
+       fbs_expr clock' (append_try_vars_to_env vl2 [exclass_to_value (fst (fst ex)); snd (fst ex); snd ex] env) id' e3 eff'
      | r => r
      end
   end
