src/Core_Erlang_Automated_Exception_Tests.v
@@ -15,7 +15,7 @@ Import ListNotations.
 *)
 Example eval_exception_call_fbs :
   (forall (env : Environment) (eff : SideEffectList) (id : nat), 
-  fbs_expr env id (ECall "+" [^ELit (Integer 5); ^ETuple []]) eff 1000 = Result id (inr (badarith (VCons (VLit (Integer 5)) (VTuple [])))) eff).
+  fbs_expr 1000 env id (ECall "+" [^ELit (Integer 5); ^ETuple []]) eff = Result id (inr (badarith (VCons (VLit (Integer 5)) (VTuple [])))) eff).
 Proof.
   intros. simpl. reflexivity.
 Qed.
@@ -32,7 +32,7 @@ Qed.
 
 
 Example exception_var_fbs :
-  fbs_expr [] 0 (EVar "X"%string) [] 1000 = Result 0 (inr novar) [].
+  fbs_expr 1000 [] 0 (EVar "X"%string) [] = Result 0 (inr novar) [].
 Proof.
   simpl. reflexivity.
 Qed.
@@ -47,10 +47,9 @@ Proof.
 Qed.
 
 Example exception_list_hd_fbs :
-  fbs_expr [] 0 
+  fbs_expr 1000 [] 0 
   (ECons (ECall "+" [^ELit (Integer 5); ^ETuple []]) (ELit (Atom "error"%string))) 
-  [] 1000
-  = Result 0 (inr (badarith (VCons (VLit (Integer 5)) (VTuple [])))) [].
+  [] = Result 0 (inr (badarith (VCons (VLit (Integer 5)) (VTuple [])))) [].
 Proof.
   simpl. reflexivity.
 Qed.
@@ -64,7 +63,7 @@ Proof.
 Qed.
 
 Example exception_list_tl_fbs : 
-  fbs_expr [] 0 (ECons (ELit (Atom "error"%string)) (ECons (ECall "+" [^ELit (Integer 5); ^ETuple []]) (ENil))) [] 1000
+  fbs_expr 1000 [] 0 (ECons (ELit (Atom "error"%string)) (ECons (ECall "+" [^ELit (Integer 5); ^ETuple []]) (ENil))) []
 =
   Result 0 (inr (badarith (VCons (VLit (Integer 5)) (VTuple [])))) [].
 Proof.
@@ -80,7 +79,7 @@ Proof.
 Qed.
 
 Example exception_tuple_fbs : 
-  fbs_expr [] 0 (ETuple [^ELit (Atom "error"%string) ; ^ELit (Atom "error"%string); ^ECall "+" [^ELit (Integer 5); ^ETuple []]]) [] 1000
+  fbs_expr 1000 [] 0 (ETuple [^ELit (Atom "error"%string) ; ^ELit (Atom "error"%string); ^ECall "+" [^ELit (Integer 5); ^ETuple []]]) []
 =
   Result 0 (inr (badarith (VCons (VLit (Integer 5)) (VTuple [])))) [].
 Proof.
@@ -96,11 +95,12 @@ Proof.
 Qed.
 
 Example try_eval_fbs : 
-  fbs_expr [] 0 (ETry (ETuple []) ["X"%string]
+  fbs_expr 1000 [] 0 
+               (ETry (ETuple []) ["X"%string]
                (ELit (Atom "ok"%string)) 
                ["Ex1"%string; "Ex2"%string; "Ex3"%string]
                (ELit (Atom "error"%string)))
-  [] 1000
+  []
 =
   Result 0 (inl [ok]) []
 .
@@ -122,11 +122,12 @@ Proof.
 Qed.
 
 Example try_eval_catch_fbs : 
-  fbs_expr [] 0 (ETry (ECall "+" [^ELit (Integer 5); ^ETuple []]) ["X"%string]
+  fbs_expr 1000 [] 0 
+               (ETry (ECall "+" [^ELit (Integer 5); ^ETuple []]) ["X"%string]
                (ELit (Atom "ok"%string))
                ["Ex1"%string; "Ex2"%string; "Ex3"%string]
                (ELit (Atom "error"%string)))
-  [] 1000
+  []
 =
   Result 0 (inl [VLit (Atom "error"%string)]) []
 .
@@ -148,11 +149,12 @@ Proof.
 Qed.
 
 Example try_eval_exception_fbs : 
-  fbs_expr [] 0 (ETry (ECall "+" [^ELit (Integer 5); ^ETuple []]) ["X"%string]
+  fbs_expr 1000 [] 0 
+               (ETry (ECall "+" [^ELit (Integer 5); ^ETuple []]) ["X"%string]
                (ELit (Atom "ok"%string))
                ["Ex1"%string; "Ex2"%string; "Ex3"%string]
                (ECall "+" [^ELit (Integer 5); ^ETuple []]))
-  [] 1000
+  []
 =
   Result 0 (inr (badarith (VCons (VLit (Integer 5)) (VTuple [])))) []
 .
@@ -174,11 +176,12 @@ Proof.
 Qed.
 
 Example try_eval_exception2_fbs : 
-  fbs_expr [] 0 (ETry (ETuple []) ["X"%string]
+  fbs_expr 1000 [] 0 
+               (ETry (ETuple []) ["X"%string]
                (ECall "+" [^ELit (Integer 5); ^ETuple []])
                ["Ex1"%string; "Ex2"%string; "Ex3"%string]
                (ELit (Atom "error"%string)))
-  [] 1000
+  []
 =
   Result 0 (inr (badarith (VCons (VLit (Integer 5)) (VTuple [])))) []
 .
@@ -200,8 +203,8 @@ Proof.
 Qed.
 
 Example eval_case_pat_ex_fbs :
-  fbs_expr [] 0 (ECase (ECall "+" [^ELit (Integer 5); ^ETuple []])
-                 [([PVar "X"%string], ^ELit (Atom "true"), ^ELit (Integer 1))]) [] 1000
+  fbs_expr 1000 [] 0 (ECase (ECall "+" [^ELit (Integer 5); ^ETuple []])
+                 [([PVar "X"%string], ^ELit (Atom "true"), ^ELit (Integer 1))]) []
 =
   Result 0 (inr (badarith (VCons (VLit (Integer 5)) (VTuple [])))) [].
 Proof.
@@ -218,10 +221,10 @@ Proof.
 Qed.
 
 Example eval_case_clause_ex_fbs :
-  fbs_expr [(inl "Y"%string, VLit (Integer 2))] 0
+  fbs_expr 1000 [(inl "Y"%string, VLit (Integer 2))] 0
      (ECase (EVar "Y"%string)
           [([PLit (Integer 1)], ^ELit (Atom "true"), ^ELit (Integer 1)); 
-           ([PVar "Z"%string], ^ELit (Atom "false"), ^ELit (Integer 2))]) [] 1000
+           ([PVar "Z"%string], ^ELit (Atom "false"), ^ELit (Integer 2))]) []
 =
   Result 0 (inr (if_clause)) [].
 Proof.
@@ -240,7 +243,7 @@ Proof.
 Qed.
 
 Example call_eval_body_ex_fbs : 
-  fbs_expr [] 0 (ECall "+"%string []) [] 1000
+  fbs_expr 1000 [] 0 (ECall "+"%string []) []
 =
   Result 0 (inr (undef (VLit (Atom "+")))) [].
 Proof.
@@ -256,7 +259,7 @@ Proof.
 Qed.
 
 Example call_eval_body_ex2_fbs :
-  fbs_expr [] 0 (ECall "+"%string [^ELit (Integer 5); ^ETuple []]) [] 1000
+  fbs_expr 1000 [] 0 (ECall "+"%string [^ELit (Integer 5); ^ETuple []]) []
 =
   Result 0 (inr (badarith (VCons (VLit (Integer 5)) (VTuple [])))) [].
 Proof.
@@ -272,7 +275,7 @@ Proof.
 Qed.
 
 Example call_eval_param_ex_fbs :
-  fbs_expr [] 0 (ECall "+"%string [^ELit (Integer 5); ^ECall "+" [^ELit (Integer 5); ^ETuple []]]) [] 1000
+  fbs_expr 1000 [] 0 (ECall "+"%string [^ELit (Integer 5); ^ECall "+" [^ELit (Integer 5); ^ETuple []]]) []
 =
   Result 0 (inr (badarith (VCons (VLit (Integer 5)) (VTuple [])))) [].
 Proof.
@@ -288,8 +291,8 @@ Proof.
 Qed.
 
 Example let_eval_exception_params_fbs :
-  fbs_expr [] 0 (ELet ["X"%string; "Y"%string] 
-               (EValues [ELit (Integer 5); ECall "+" [^ELit (Integer 5); ^ETuple []]]) (ETuple [])) [] 1000
+  fbs_expr 1000 [] 0 (ELet ["X"%string; "Y"%string] 
+               (EValues [ELit (Integer 5); ECall "+" [^ELit (Integer 5); ^ETuple []]]) (ETuple [])) []
 =
   Result 0 (inr (badarith (VCons (VLit (Integer 5)) (VTuple [])))) [].
 Proof.
@@ -306,8 +309,8 @@ Proof.
 Qed.
 
 Example let_eval_exception_body_fbs :
-  fbs_expr [] 0 (ELet ["X"%string; "Y"%string] (EValues [ELit (Integer 5); ELit (Integer 5)])
-               (ECall "+" [^ELit (Integer 5); ^ETuple []])) [] 1000
+  fbs_expr 1000 [] 0 (ELet ["X"%string; "Y"%string] (EValues [ELit (Integer 5); ELit (Integer 5)])
+               (ECall "+" [^ELit (Integer 5); ^ETuple []])) []
 =
   Result 0 (inr (badarith (VCons (VLit (Integer 5)) (VTuple [])))) [].
 Proof.
@@ -324,7 +327,7 @@ Proof.
 Qed.
 
 Example apply_eval_exception_closure_fbs :
-  fbs_expr [] 0 (EApp (ELit (Integer 4)) [^ELit (Integer 5); ^ELit (Integer 5)]) [] 1000
+  fbs_expr 1000 [] 0 (EApp (ELit (Integer 4)) [^ELit (Integer 5); ^ELit (Integer 5)]) []
 =
   Result 0 (inr (badfun (VLit (Integer 4)))) [].
 Proof.
@@ -340,7 +343,7 @@ Proof.
 Qed.
 
 Example apply_eval_exception_closure2_fbs :
-  fbs_expr [] 0 (EApp (ECall "+" [^ELit (Integer 5); ^ETuple []]) [^ELit (Integer 5); ^ELit (Integer 5)]) [] 1000
+  fbs_expr 1000 [] 0 (EApp (ECall "+" [^ELit (Integer 5); ^ETuple []]) [^ELit (Integer 5); ^ELit (Integer 5)]) []
 =
   Result 0 (inr (badarith (VCons (VLit (Integer 5)) (VTuple [])))) [].
 Proof.
@@ -356,8 +359,8 @@ Proof.
 Qed.
 
 Example apply_eval_exception_param_fbs :
-  fbs_expr [(inl "X"%string, VClos [] [] 0 [] (ELit (Integer 4)))] 1
-    (EApp (EVar "X"%string) [^ECall "+" [^ELit (Integer 5); ^ETuple []]]) [] 1000
+  fbs_expr 1000 [(inl "X"%string, VClos [] [] 0 [] (ELit (Integer 4)))] 1
+    (EApp (EVar "X"%string) [^ECall "+" [^ELit (Integer 5); ^ETuple []]]) []
 =
   Result 1 (inr (badarith (VCons (VLit (Integer 5)) (VTuple [])))) [].
 Proof.
@@ -374,8 +377,8 @@ Proof.
 Qed.
 
 Example apply_eval_exception_param_count_fbs :
-  fbs_expr [(inl "X"%string, VClos [] [] 0 [] (ELit (Integer 4)))] 1
-   (EApp (EVar "X"%string) [^ELit (Integer 2)]) [] 1000
+  fbs_expr 1000 [(inl "X"%string, VClos [] [] 0 [] (ELit (Integer 4)))] 1
+   (EApp (EVar "X"%string) [^ELit (Integer 2)]) []
 =
   Result 1 (inr (badarity (VClos [] [] 0 [] (ELit (Integer 4))))) [].
 Proof.
@@ -392,8 +395,8 @@ Proof.
 Qed.
 
 Example apply_eval_exception_body_fbs :
-  fbs_expr [(inl "X"%string, VClos [] [] 0 [] (ECall "+" [^ELit (Integer 5); ^ETuple []]))] 1
-   (EApp (EVar "X"%string) []) [] 1000
+  fbs_expr 1000 [(inl "X"%string, VClos [] [] 0 [] (ECall "+" [^ELit (Integer 5); ^ETuple []]))] 1
+   (EApp (EVar "X"%string) []) []
 =
   Result 1 (inr (badarith (VCons (VLit (Integer 5)) (VTuple [])))) [].
 Proof.
@@ -410,7 +413,7 @@ Proof.
 Qed.
 
 Example letrec_exception_fbs : 
-  fbs_expr [] 0 (ELetRec [(("fun1"%string, 0), ([], ^ELit (Atom "error"%string)))] (ECall "+" [^ELit (Integer 5); ^ETuple []])) [] 1000
+  fbs_expr 1000 [] 0 (ELetRec [(("fun1"%string, 0), ([], ^ELit (Atom "error"%string)))] (ECall "+" [^ELit (Integer 5); ^ETuple []])) []
 =
   Result 1 (inr (badarith (VCons (VLit (Integer 5)) (VTuple [])))) [].
 Proof.
@@ -426,10 +429,10 @@ Proof.
 Qed.
 
 Example map_eval_ex_key_fbs :
-  fbs_expr [] 0 (EMap [(^ELit (Atom "error"%string), ^ ELit (Atom "error"%string)); 
+  fbs_expr 1000 [] 0 (EMap [(^ELit (Atom "error"%string), ^ ELit (Atom "error"%string)); 
                 (^ELit (Atom "error"%string), ^ELit (Atom "error"%string));
                 (^ECall "+" [^ELit (Integer 5); ^ETuple []], ^ELit (Atom "error"%string));
-                (^ELit (Atom "error"%string), ^ELit (Atom "error"%string))]) [] 1000
+                (^ELit (Atom "error"%string), ^ELit (Atom "error"%string))]) []
 =
   Result 0 (inr (badarith (VCons (VLit (Integer 5)) (VTuple [])))) [].
 Proof.
@@ -448,10 +451,11 @@ Proof.
 Qed.
 
 Example map_eval_ex_val_fbs :
-  fbs_expr [] 0 (EMap [(^ELit (Atom "error"%string), ^ELit (Atom "error"%string)); 
+  fbs_expr 1000 [] 0 
+                (EMap [(^ELit (Atom "error"%string), ^ELit (Atom "error"%string)); 
                 (^ELit (Atom "error"%string), ^ECall "+" [^ELit (Integer 5); ^ETuple []]);
                 (^ELit (Atom "error"%string), ^ELit (Atom "error"%string));
-                (^ELit (Atom "error"%string), ^ELit (Atom "error"%string))]) [] 1000
+                (^ELit (Atom "error"%string), ^ELit (Atom "error"%string))]) []
 =
   Result 0 (inr (badarith (VCons (VLit (Integer 5)) (VTuple [])))) [].
 Proof.
@@ -470,8 +474,8 @@ Proof.
 Qed.
 
 Example seq_eval_ex_1_fbs :
-  fbs_expr [] 0 (ESeq (ECall "+" [^ELit (Integer 5); ^ETuple []])
-                (ELit (Integer 42))) [] 1000
+  fbs_expr 1000 [] 0 (ESeq (ECall "+" [^ELit (Integer 5); ^ETuple []])
+                (ELit (Integer 42))) []
 =
   Result 0 (inr (badarith (VCons (VLit (Integer 5)) (VTuple [])))) [].
 Proof.
@@ -489,8 +493,8 @@ Proof.
 Qed.
 
 Example seq_eval_ex_2_fbs :
-  fbs_expr [] 0 (ESeq (ELit (Integer 42))
-                (ECall "+" [^ELit (Integer 5); ^ETuple []])) [] 1000
+  fbs_expr 1000 [] 0 (ESeq (ELit (Integer 42))
+                (ECall "+" [^ELit (Integer 5); ^ETuple []])) []
 =
   Result 0 (inr (badarith (VCons (VLit (Integer 5)) (VTuple [])))) [] .
 Proof.
@@ -508,7 +512,7 @@ Proof.
 Qed.
 
 Example map_eval_ex_val2_fbs :
-  fbs_expr [] 0 (EMap [(^ELit (Atom "error"%string), ^ELit (Atom "error"%string)); 
+  fbs_expr 1000 [] 0 (EMap [(^ELit (Atom "error"%string), ^ELit (Atom "error"%string)); 
                 (^ELit (Atom "error"%string), ^ELit (Atom "error"%string));
                 (^ELit (Atom "error"%string), ^ELit (Atom "error"%string));
                 (^ELit (Atom "error"%string), ^EMap [(^ELit (Atom "error"%string), ^ELit (Atom "error"%string)); 
@@ -529,7 +533,7 @@ Example map_eval_ex_val2_fbs :
                 (^EMap [(^ELit (Atom "error"%string), ^ELit (Atom "error"%string)); 
                 (^ELit (Atom "error"%string), ^ECall "+" [^ELit (Integer 5); ^ETuple []]);
                 (^ELit (Atom "error"%string), ^ELit (Atom "error"%string));
-                (^ELit (Atom "error"%string), ^ELit (Atom "error"%string))], ^ECall "+" [^ELit (Integer 5); ^ETuple []])])])])])])]) [] 1000
+                (^ELit (Atom "error"%string), ^ELit (Atom "error"%string))], ^ECall "+" [^ELit (Integer 5); ^ETuple []])])])])])])]) []
 =
   Result 0 (inr (badarith (VCons (VLit (Integer 5)) (VTuple [])))) [].
 Proof.
